ulib/experimental/Steel.Effect.Atomic.fst
@@ -71,46 +71,7 @@ val elim_star_pat (p q:slprop) (m:hmem (p `star` q))
     [SMTPat (interp (p `star` q) m)]
 let elim_star_pat = elim_star
 
-module G = FStar.Ghost
-
-val id_elim_star (p q:slprop) (m:mem)
-  : Pure (G.erased mem & G.erased mem)
-         (requires (interp (p `star` q) m))
-         (ensures (fun (ml, mr) -> disjoint ml mr
-                              /\ m == join ml mr
-                              /\ interp p ml
-                              /\ interp q mr))
-
-let id_elim_star p q m =
-  let starprop (ml:mem) (mr:mem) =
-      disjoint ml mr
-    /\ m == join ml mr
-    /\ interp p ml
-    /\ interp q mr
-  in
-  let p1 : mem -> prop = fun ml -> (exists mr. starprop ml mr) in
-  let ml = IndefiniteDescription.indefinite_description_tot _ p1 in
-  let starpropml mr : prop = starprop ml mr in // this prop annotation seems needed
-  let mr = IndefiniteDescription.indefinite_description_tot _ starpropml in
-  (ml, mr)
-
-val id_elim_exists (#a:Type) (p : a -> slprop) (m:mem)
-  : Pure (G.erased a)
-         (requires (interp (h_exists p) m))
-         (ensures (fun x -> interp (p x) m))
-
-let id_elim_exists #a p m =
-  let existsprop (x:a) =
-    interp (p x) m
-  in
-  Steel.Memory.elim_h_exists p m;
-  let x = IndefiniteDescription.indefinite_description_tot _ existsprop in
-  x
-
-// let witness_invariant #a (p : a -> slprop) =
-//   forall x y m. interp (p x) m /\ interp (p y) m ==> x == y
-
-let witness_h_exists (#a:Type) (#opened:_) (#p:(a -> slprop){witness_invariant p}) ()
+let witness_h_exists (#a:Type) (#opened:_) (#p:(a -> slprop){is_frame_monotonic p}) ()
   : SteelAtomic (Ghost.erased a) opened unobservable
                 (h_exists p) (fun x -> p x)
   =
