ulib/experimental/Steel.HigherReference.fst
@@ -103,16 +103,31 @@ let pts_to_ref_injective
                               (Some (Ghost.reveal v1, p1))
                               m
                               
-let pts_to_witinv (#a:Type) (r:ref a) (p:perm) : Lemma (witness_invariant (pts_to r p)) =
+let pts_to_framon (#a:Type) (r:ref a) (p:perm) : Lemma (is_frame_monotonic #a (fun v -> pts_to r p v)) =
+  let aux (x y : a) (m:mem) (f:slprop)
+    : Lemma (requires (interp (pts_to r p x `star` f) m /\ interp (pts_to r p y) m))
+            (ensures  (slimp (pts_to r p x) (pts_to r p y)))
+    =
+    let (ml, mr) = id_elim_star (pts_to r p x) f m in
+    assert (interp (pts_to r p x) ml);
+    assert (interp (pts_to r p x) m);
+    assert (interp (pts_to_raw r p y) m);
+    assert (interp (Mem.pts_to r (Some (Ghost.reveal x, p))) m);
+    assert (interp (Mem.pts_to r (Some (Ghost.reveal y, p))) m);
+    Mem.pts_to_join r (Some (Ghost.reveal x, p)) (Some (Ghost.reveal y, p)) m;
+    ()
+  in
+  Classical.forall_intro_4 (fun x y m -> Classical.move_requires (aux x y m))
+
+let pts_to_witinv (#a:Type) (r:ref a) (p:perm) : Lemma (witness_invariant #a (fun v -> pts_to r p v)) =
   let aux (x y : a) (m:mem)
     : Lemma (requires (interp (pts_to r p x) m /\ interp (pts_to r p y) m))
             (ensures  (x == y))
     =
-    pts_to_join r (Some (Ghost.reveal x, p)) (Some (Ghost.reveal y, p)) m;
-    ()
+    Mem.pts_to_join r (Some (Ghost.reveal x, p)) (Some (Ghost.reveal y, p)) m
   in
   Classical.forall_intro_3 (fun x y -> Classical.move_requires (aux x y))
-
+  
 let drop (p:slprop)
   : SteelT unit p (fun _ -> emp)
   = lift_atomic_to_steelT (fun _ ->
@@ -187,8 +202,9 @@ let read (#a:Type) (#p:perm) (#v:erased a) (r:ref a)
 
 let read_refine (#a:Type) (#p:perm) (q:a -> slprop) (r:ref a)
   : SteelT a (h_exists (fun (v:a) -> pts_to r p v `star` q v))
-             (fun v -> pts_to r p v `star` q v)
+             (fun (v:a) -> pts_to r p v `star` q v)
   = pts_to_witinv r p;
+    star_is_witinv_left (fun (v:a) -> pts_to r p v) q;
     let vs = SB.witness_h_exists () in
     SB.h_assert (pts_to r p vs `star` q vs);
     let v = SB.frame (fun _ -> read #a #p #vs r) _ in
