ulib/FStar.PCM.fst
@@ -100,6 +100,13 @@ let compatible_refl
   pcm.is_unit x;
   pcm.comm x pcm.p.one;
   assert (op pcm pcm.p.one x == x)
+  
+(** Compatibility is transitive *)
+let compatible_trans
+  (#a: Type u#a) (pcm:pcm a) (x y z:a)
+  : Lemma (requires (compatible pcm x y /\ compatible pcm y z))
+          (ensures (compatible pcm x z))
+  = Classical.forall_intro_3 pcm.assoc
 
 (**
   Helper function to get access to the existentially quantified frame between two compatible
